isabelle/OpSet.thy
@@ -170,42 +170,42 @@ next
 qed
 
 
-subsection\<open>The spec\_ops predicate\<close>
+subsection\<open>The \isa{spec-ops} predicate\<close>
 
-text\<open>The spec\_ops predicate describes a list of (ID, operation) pairs that
+text\<open>The \isa{spec-ops} predicate describes a list of (ID, operation) pairs that
 corresponds to the linearisation of an OpSet, and which we use for sequentially
-interpreting the OpSet. A list satisfies spec\_ops iff it is sorted in ascending
+interpreting the OpSet. A list satisfies \isa{spec-ops} iff it is sorted in ascending
 order of IDs, if the IDs are unique, and if every operation's dependencies have
 lower IDs than the operation itself. A list is implicitly finite in Isabelle/HOL.
 These requirements correspond to the OpSet definition above, and indeed we prove
-later that every OpSet has a linearisation that satisfies spec\_ops.\<close>
+later that every OpSet has a linearisation that satisfies \isa{spec-ops}.\<close>
 
-definition spec_ops :: "('oper \<Rightarrow> 'oid set) \<Rightarrow> ('oid::{linorder} \<times> 'oper) list \<Rightarrow> bool" where
-  "spec_ops deps ops \<equiv> (sorted (map fst ops) \<and> distinct (map fst ops) \<and>
+definition spec_ops :: "('oid::{linorder} \<times> 'oper) list \<Rightarrow> ('oper \<Rightarrow> 'oid set) \<Rightarrow> bool" where
+  "spec_ops ops deps \<equiv> (sorted (map fst ops) \<and> distinct (map fst ops) \<and>
            (\<forall>oid oper ref. (oid, oper) \<in> set ops \<and> ref \<in> deps oper \<longrightarrow> ref < oid))"
 
 lemma spec_ops_empty:
-  shows "spec_ops deps []"
+  shows "spec_ops [] deps"
 by (simp add: spec_ops_def)
 
 lemma spec_ops_distinct:
-  assumes "spec_ops deps ops"
+  assumes "spec_ops ops deps"
   shows "distinct ops"
 using assms distinct_map spec_ops_def by blast
 
 lemma spec_ops_distinct_fst:
-  assumes "spec_ops deps ops"
+  assumes "spec_ops ops deps"
   shows "distinct (map fst ops)"
 using assms by (simp add: spec_ops_def)
 
 lemma spec_ops_sorted:
-  assumes "spec_ops deps ops"
+  assumes "spec_ops ops deps"
   shows "sorted (map fst ops)"
 using assms by (simp add: spec_ops_def)
 
 lemma spec_ops_rem_cons:
-  assumes "spec_ops deps (x # xs)"
-  shows "spec_ops deps xs"
+  assumes "spec_ops (x # xs) deps"
+  shows "spec_ops xs deps"
 proof -
   have "sorted (map fst (x # xs))" and "distinct (map fst (x # xs))"
     using assms spec_ops_def by blast+
@@ -213,13 +213,13 @@ proof -
     by (simp add: sorted_Cons)
   moreover have "\<forall>oid oper ref. (oid, oper) \<in> set xs \<and> ref \<in> deps oper \<longrightarrow> ref < oid"
     by (meson assms set_subset_Cons spec_ops_def subsetCE)
-  ultimately show "spec_ops deps xs"
+  ultimately show "spec_ops xs deps"
     by (simp add: spec_ops_def)
 qed
 
 lemma spec_ops_rem_last:
-  assumes "spec_ops deps (xs @ [x])"
-  shows "spec_ops deps xs"
+  assumes "spec_ops (xs @ [x]) deps"
+  shows "spec_ops xs deps"
 proof -
   have "sorted (map fst (xs @ [x]))" and "distinct (map fst (xs @ [x]))"
     using assms spec_ops_def by blast+
@@ -227,31 +227,31 @@ proof -
     by (auto simp add: sorted_append distinct_butlast distinct_map)
   moreover have "\<forall>oid oper ref. (oid, oper) \<in> set xs \<and> ref \<in> deps oper \<longrightarrow> ref < oid"
     by (metis assms butlast_snoc in_set_butlastD spec_ops_def)
-  ultimately show "spec_ops deps xs"
+  ultimately show "spec_ops xs deps"
     by (simp add: spec_ops_def)
 qed
 
 lemma spec_ops_remove1:
-  assumes "spec_ops deps xs"
-  shows "spec_ops deps (remove1 x xs)"
+  assumes "spec_ops xs deps"
+  shows "spec_ops (remove1 x xs) deps"
 using assms distinct_map_fst_remove1 spec_ops_def
 by (metis notin_set_remove1 sorted_map_remove1 spec_ops_def)
 
 lemma spec_ops_ref_less:
-  assumes "spec_ops deps xs"
+  assumes "spec_ops xs deps"
     and "(oid, oper) \<in> set xs"
     and "r \<in> deps oper"
   shows "r < oid"
 using assms spec_ops_def by force
 
 lemma spec_ops_ref_less_last:
-  assumes "spec_ops deps (xs @ [(oid, oper)])"
+  assumes "spec_ops (xs @ [(oid, oper)]) deps"
     and "r \<in> deps oper"
   shows "r < oid"
 using assms spec_ops_ref_less by fastforce
 
 lemma spec_ops_id_inc:
-  assumes "spec_ops deps (xs @ [(oid, oper)])"
+  assumes "spec_ops (xs @ [(oid, oper)]) deps"
     and "x \<in> set (map fst xs)"
   shows "x < oid"
 proof -
@@ -268,10 +268,10 @@ proof -
 qed
 
 lemma spec_ops_add_last:
-  assumes "spec_ops deps xs"
+  assumes "spec_ops xs deps"
     and "\<forall>i \<in> set (map fst xs). i < oid"
     and "\<forall>ref \<in> deps oper. ref < oid"
-  shows "spec_ops deps (xs @ [(oid, oper)])"
+  shows "spec_ops (xs @ [(oid, oper)]) deps"
 proof -
   have "sorted ((map fst xs) @ [oid])"
     using assms sorted_append spec_ops_sorted by fastforce
@@ -281,27 +281,27 @@ proof -
     using assms(1) spec_ops_def by fastforce
   hence "\<forall>i opr r. (i, opr) \<in> set (xs @ [(oid, oper)]) \<and> r \<in> deps opr \<longrightarrow> r < i"
     using assms(3) by auto
-  ultimately show "spec_ops deps (xs @ [(oid, oper)])"
+  ultimately show "spec_ops (xs @ [(oid, oper)]) deps"
     by (simp add: spec_ops_def)
 qed
 
 lemma spec_ops_add_any:
-  assumes "spec_ops deps (xs @ ys)"
+  assumes "spec_ops (xs @ ys) deps"
     and "\<forall>i \<in> set (map fst xs). i < oid"
     and "\<forall>i \<in> set (map fst ys). oid < i"
     and "\<forall>ref \<in> deps oper. ref < oid"
-  shows "spec_ops deps (xs @ [(oid, oper)] @ ys)"
+  shows "spec_ops (xs @ [(oid, oper)] @ ys) deps"
 using assms proof(induction ys rule: rev_induct)
   case Nil
-  then show "spec_ops deps (xs @ [(oid, oper)] @ [])"
+  then show "spec_ops (xs @ [(oid, oper)] @ []) deps"
     by (simp add: spec_ops_add_last)
 next
   case (snoc y ys)
-  have IH: "spec_ops deps (xs @ [(oid, oper)] @ ys)"
+  have IH: "spec_ops (xs @ [(oid, oper)] @ ys) deps"
   proof -
-    from snoc have "spec_ops deps (xs @ ys)"
+    from snoc have "spec_ops (xs @ ys) deps"
       by (metis append_assoc spec_ops_rem_last)
-    thus "spec_ops deps (xs @ [(oid, oper)] @ ys)"
+    thus "spec_ops (xs @ [(oid, oper)] @ ys) deps"
       using assms(2) snoc by auto
   qed
   obtain yi yo where y_pair: "y = (yi, yo)"
@@ -346,12 +346,12 @@ next
     ultimately show ?thesis
       using y_pair by auto
   qed
-  ultimately show "spec_ops deps (xs @ [(oid, oper)] @ ys @ [y])"
+  ultimately show "spec_ops (xs @ [(oid, oper)] @ ys @ [y]) deps"
     using spec_ops_def by blast
 qed
 
 lemma spec_ops_split:
-  assumes "spec_ops deps xs"
+  assumes "spec_ops xs deps"
     and "oid \<notin> set (map fst xs)"
   shows "\<exists>pre suf. xs = pre @ suf \<and>
             (\<forall>i \<in> set (map fst pre). i < oid) \<and>
@@ -398,14 +398,14 @@ lemma spec_ops_exists_base:
   assumes "finite ops"
     and "\<And>oid op1 op2. (oid, op1) \<in> ops \<Longrightarrow> (oid, op2) \<in> ops \<Longrightarrow> op1 = op2"
     and "\<And>oid oper ref. (oid, oper) \<in> ops \<Longrightarrow> ref \<in> deps oper \<Longrightarrow> ref < oid"
-  shows "\<exists>op_list. set op_list = ops \<and> spec_ops deps op_list"
+  shows "\<exists>op_list. set op_list = ops \<and> spec_ops op_list deps"
 using assms proof(induct ops rule: Finite_Set.finite_induct_select)
   case empty
-  then show "\<exists>op_list. set op_list = {} \<and> spec_ops deps op_list"
+  then show "\<exists>op_list. set op_list = {} \<and> spec_ops op_list deps"
     by (simp add: spec_ops_empty)
 next
   case (select subset)
-  from this obtain op_list where "set op_list = subset" and "spec_ops deps op_list"
+  from this obtain op_list where "set op_list = subset" and "spec_ops op_list deps"
     using assms by blast
   moreover obtain oid oper where select: "(oid, oper) \<in> ops - subset"
     using select.hyps(1) by auto
@@ -420,17 +420,17 @@ next
     using spec_ops_split calculation by (metis (no_types, lifting) set_map)
   moreover have "set (pre @ [(oid, oper)] @ suf) = insert (oid, oper) subset"
     using calculation by auto
-  moreover have "spec_ops deps (pre @ [(oid, oper)] @ suf)"
+  moreover have "spec_ops (pre @ [(oid, oper)] @ suf) deps"
     using calculation spec_ops_add_any assms(3) by (metis DiffD1)
   ultimately show ?case by blast
 qed
 
-text\<open>Proof that for any given OpSet, a spec\_ops linearisation exists;
-and, conversely, for any given spec\_ops list, the set of pairs is an OpSet.\<close>
+text\<open>Proof that for any given OpSet, a \isa{spec-ops} linearisation exists;
+and, conversely, for any given \isa{spec-ops} list, the set of pairs is an OpSet.\<close>
 
 lemma spec_ops_exists:
   assumes "opset ops deps"
-  shows "\<exists>op_list. set op_list = ops \<and> spec_ops deps op_list"
+  shows "\<exists>op_list. set op_list = ops \<and> spec_ops op_list deps"
 proof -
   have "finite ops"
     using assms opset.finite_opset by force
@@ -438,12 +438,12 @@ proof -
     using assms opset.unique_oid by force
   moreover have "\<And>oid oper ref. (oid, oper) \<in> ops \<Longrightarrow> ref \<in> deps oper \<Longrightarrow> ref < oid"
     using assms opset.ref_older by force
-  ultimately show "\<exists>op_list. set op_list = ops \<and> spec_ops deps op_list"
+  ultimately show "\<exists>op_list. set op_list = ops \<and> spec_ops op_list deps"
     by (simp add: spec_ops_exists_base)
 qed
 
 lemma spec_ops_oid_unique:
-  assumes "spec_ops deps op_list"
+  assumes "spec_ops op_list deps"
     and "(oid, op1) \<in> set op_list"
     and "(oid, op2) \<in> set op_list"
   shows "op1 = op2"
@@ -468,7 +468,7 @@ using assms proof(induction op_list, simp)
 qed
 
 lemma spec_ops_is_opset:
-  assumes "spec_ops deps op_list"
+  assumes "spec_ops op_list deps"
   shows "opset (set op_list) deps"
 proof -
   have "\<And>oid op1 op2. (oid, op1) \<in> set op_list \<Longrightarrow> (oid, op2) \<in> set op_list \<Longrightarrow> op1 = op2"
@@ -482,78 +482,86 @@ proof -
 qed
 
 
-subsection\<open>The crdt\_ops predicate\<close>
+subsection\<open>The \isa{crdt-ops} predicate\<close>
 
-text\<open>Like spec\_ops, the crdt\_ops predicate describes the linearisation of
-an OpSet into a list. Like spec\_ops, it requires IDs to be unique. However,
-its other properties are different: crdt\_ops does not require operations to
+text\<open>Like \isa{spec-ops}, the \isa{crdt-ops} predicate describes the linearisation of
+an OpSet into a list. Like \isa{spec-ops}, it requires IDs to be unique. However,
+its other properties are different: \isa{crdt-ops} does not require operations to
 appear in sorted order, but instead, whenever any operation references the
 ID of a prior operation, that prior operation must appear previously in the
-crdt\_ops list. Thus, the order of operations is partially constrained:
+\isa{crdt-ops} list. Thus, the order of operations is partially constrained:
 operations must appear in causal order, but concurrent operations can be
 ordered arbitrarily.
 
 This list describes the operation sequence as it is typically applied to an
 operation-based CRDT. Applying operations in the order they appear in
-crdt\_ops requires that concurrent operations commute. For any crdt\_ops
-operation sequence, there is a permutation that satisfies the spec\_ops
+\isa{crdt-ops} requires that concurrent operations commute. For any \isa{crdt-ops}
+operation sequence, there is a permutation that satisfies the \isa{spec-ops}
 predicate. Thus, to check whether a CRDT satisfies its sequential specification,
-we can prove that interpreting any crdt\_ops operation sequence with the
+we can prove that interpreting any \isa{crdt-ops} operation sequence with the
 commutative operation interpretation results in the same end result as
-interpreting the spec\_ops permutation of that operation sequence with the
+interpreting the \isa{spec-ops} permutation of that operation sequence with the
 sequential operation interpretation.\<close>
 
-inductive crdt_ops :: "('oper \<Rightarrow> 'oid set) \<Rightarrow> ('oid::{linorder} \<times> 'oper) list \<Rightarrow> bool" where
-  "crdt_ops deps []" |
-  "\<lbrakk>crdt_ops deps xs;
+inductive crdt_ops :: "('oid::{linorder} \<times> 'oper) list \<Rightarrow> ('oper \<Rightarrow> 'oid set) \<Rightarrow> bool" where
+  "crdt_ops [] deps" |
+  "\<lbrakk>crdt_ops xs deps;
     oid \<notin> set (map fst xs);
     \<forall>ref \<in> deps oper. ref \<in> set (map fst xs) \<and> ref < oid
-   \<rbrakk> \<Longrightarrow> crdt_ops deps (xs @ [(oid, oper)])"
+   \<rbrakk> \<Longrightarrow> crdt_ops (xs @ [(oid, oper)]) deps"
 
-inductive_cases crdt_ops_last: "crdt_ops deps (xs @ [x])"
+inductive_cases crdt_ops_last: "crdt_ops (xs @ [x]) deps"
 
 lemma crdt_ops_intro:
   assumes "\<And>r. r \<in> deps oper \<Longrightarrow> r \<in> fst ` set xs \<and> r < oid"
     and "oid \<notin> fst ` set xs"
-    and "crdt_ops deps xs"
-  shows "crdt_ops deps (xs @ [(oid, oper)])"
+    and "crdt_ops xs deps"
+  shows "crdt_ops (xs @ [(oid, oper)]) deps"
 using assms crdt_ops.simps by force
 
 lemma crdt_ops_rem_last:
-  assumes "crdt_ops deps (xs @ [x])"
-  shows "crdt_ops deps xs"
+  assumes "crdt_ops (xs @ [x]) deps"
+  shows "crdt_ops xs deps"
 using assms crdt_ops.cases snoc_eq_iff_butlast by blast
 
 lemma crdt_ops_ref_less:
-  assumes "crdt_ops deps xs"
+  assumes "crdt_ops xs deps"
     and "(oid, oper) \<in> set xs"
     and "r \<in> deps oper"
   shows "r < oid"
 using assms by (induction rule: crdt_ops.induct, auto)
 
 lemma crdt_ops_ref_less_last:
-  assumes "crdt_ops deps (xs @ [(oid, oper)])"
+  assumes "crdt_ops (xs @ [(oid, oper)]) deps"
     and "r \<in> deps oper"
   shows "r < oid"
 using assms crdt_ops_ref_less by fastforce
 
-lemma crdt_ops_distinct:
-  assumes "crdt_ops deps xs"
-  shows "distinct xs"
-using assms by (induction xs, force+)
-
 lemma crdt_ops_distinct_fst:
-  assumes "crdt_ops deps xs"
+  assumes "crdt_ops xs deps"
   shows "distinct (map fst xs)"
-using assms by (induction xs, auto)
+using assms proof (induction xs rule: List.rev_induct, simp)
+  case (snoc x xs)
+  hence "distinct (map fst xs)"
+    using crdt_ops_last by blast
+  moreover have "fst x \<notin> set (map fst xs)"
+    using snoc by (metis crdt_ops_last fstI image_set)
+  ultimately show "distinct (map fst (xs @ [x]))"
+    by simp
+qed
+
+lemma crdt_ops_distinct:
+  assumes "crdt_ops xs deps"
+  shows "distinct xs"
+using assms crdt_ops_distinct_fst distinct_map by blast
 
 lemma crdt_ops_unique_last:
-  assumes "crdt_ops deps (xs @ [(oid, oper)])"
+  assumes "crdt_ops (xs @ [(oid, oper)]) deps"
   shows "oid \<notin> set (map fst xs)"
 using assms crdt_ops.cases by blast
 
 lemma crdt_ops_unique_mid:
-  assumes "crdt_ops deps (xs @ [(oid, oper)] @ ys)"
+  assumes "crdt_ops (xs @ [(oid, oper)] @ ys) deps"
   shows "oid \<notin> set (map fst xs) \<and> oid \<notin> set (map fst ys)"
 using assms proof(induction ys rule: rev_induct)  
   case Nil
@@ -574,7 +582,7 @@ next
 qed
 
 lemma crdt_ops_ref_exists:
-  assumes "crdt_ops deps (pre @ (oid, oper) # suf)"
+  assumes "crdt_ops (pre @ (oid, oper) # suf) deps"
     and "ref \<in> deps oper"
   shows "ref \<in> fst ` set pre"
 using assms proof(induction suf rule: List.rev_induct)
@@ -586,7 +594,7 @@ next
 qed
 
 lemma crdt_ops_no_future_ref:
-  assumes "crdt_ops deps (xs @ [(oid, oper)] @ ys)"
+  assumes "crdt_ops (xs @ [(oid, oper)] @ ys) deps"
   shows "\<And>ref. ref \<in> deps oper \<Longrightarrow> ref \<notin> fst ` set ys"
 proof -
   from assms(1) have "\<And>ref. ref \<in> deps oper \<Longrightarrow> ref \<in> set (map fst xs)"
@@ -600,25 +608,25 @@ proof -
 qed
 
 lemma crdt_ops_reorder:
-  assumes "crdt_ops deps (xs @ [(oid, oper)] @ ys)"
+  assumes "crdt_ops (xs @ [(oid, oper)] @ ys) deps"
     and "\<And>op2 r. op2 \<in> snd ` set ys \<Longrightarrow> r \<in> deps op2 \<Longrightarrow> r \<noteq> oid"
-  shows "crdt_ops deps (xs @ ys @ [(oid, oper)])"
+  shows "crdt_ops (xs @ ys @ [(oid, oper)]) deps"
 using assms proof(induction ys rule: rev_induct)
   case Nil
-  then show "crdt_ops deps (xs @ [] @ [(oid, oper)])"
+  then show "crdt_ops (xs @ [] @ [(oid, oper)]) deps"
     using crdt_ops_rem_last by auto
 next
   case (snoc y ys)
   then obtain yi yo where y_pair: "y = (yi, yo)"
     by fastforce
-  have IH: "crdt_ops deps (xs @ ys @ [(oid, oper)])"
+  have IH: "crdt_ops (xs @ ys @ [(oid, oper)]) deps"
   proof -
-    have "crdt_ops deps (xs @ [(oid, oper)] @ ys)"
+    have "crdt_ops (xs @ [(oid, oper)] @ ys) deps"
       by (metis snoc(2) append.assoc crdt_ops_rem_last)
-    thus "crdt_ops deps (xs @ ys @ [(oid, oper)])"
+    thus "crdt_ops (xs @ ys @ [(oid, oper)]) deps"
       using snoc.IH snoc.prems(2) by auto
   qed
-  have "crdt_ops deps (xs @ ys @ [y])"
+  have "crdt_ops (xs @ ys @ [y]) deps"
   proof -
     have "yi \<notin> fst ` set (xs @ [(oid, oper)] @ ys)"
       by (metis y_pair append_assoc crdt_ops_unique_last set_map snoc.prems(1))
@@ -635,9 +643,9 @@ next
       ultimately show "\<And>r. r \<in> deps yo \<Longrightarrow> r \<in> fst ` set (xs @ ys) \<and> r < yi"
         by simp
     qed
-    moreover from IH have "crdt_ops deps (xs @ ys)"
+    moreover from IH have "crdt_ops (xs @ ys) deps"
       using crdt_ops_rem_last by force
-    ultimately show "crdt_ops deps (xs @ ys @ [y])"
+    ultimately show "crdt_ops (xs @ ys @ [y]) deps"
       using y_pair crdt_ops_intro by (metis append.assoc)
   qed
   moreover have "oid \<notin> fst ` set (xs @ ys @ [y])"
@@ -648,19 +656,19 @@ next
     by (metis UnCI append_Cons image_Un set_append snoc.prems(1))
   moreover have "\<And>r. r \<in> deps oper \<Longrightarrow> r < oid"
     using IH crdt_ops_ref_less by fastforce
-  ultimately show "crdt_ops deps (xs @ (ys @ [y]) @ [(oid, oper)])"
+  ultimately show "crdt_ops (xs @ (ys @ [y]) @ [(oid, oper)]) deps"
     using crdt_ops_intro by (metis append_assoc)
 qed
 
 lemma crdt_ops_rem_middle:
-  assumes "crdt_ops deps (xs @ [(oid, ref)] @ ys)"
+  assumes "crdt_ops (xs @ [(oid, ref)] @ ys) deps"
     and "\<And>op2 r. op2 \<in> snd ` set ys \<Longrightarrow> r \<in> deps op2 \<Longrightarrow> r \<noteq> oid"
-  shows "crdt_ops deps (xs @ ys)"
+  shows "crdt_ops (xs @ ys) deps"
 using assms crdt_ops_rem_last crdt_ops_reorder append_assoc by metis
 
 lemma crdt_ops_independent_suf:
-  assumes "spec_ops deps (xs @ [(oid, oper)])"
-    and "crdt_ops deps (ys @ [(oid, oper)] @ zs)"
+  assumes "spec_ops (xs @ [(oid, oper)]) deps"
+    and "crdt_ops (ys @ [(oid, oper)] @ zs) deps"
     and "set (xs @ [(oid, oper)]) = set (ys @ [(oid, oper)] @ zs)"
   shows "\<And>op2 r. op2 \<in> snd ` set zs \<Longrightarrow> r \<in> deps op2 \<Longrightarrow> r \<noteq> oid"
 proof -
@@ -687,39 +695,39 @@ proof -
 qed
 
 lemma crdt_ops_reorder_spec:
-  assumes "spec_ops deps (xs @ [x])"
-    and "crdt_ops deps (ys @ [x] @ zs)"
+  assumes "spec_ops (xs @ [x]) deps"
+    and "crdt_ops (ys @ [x] @ zs) deps"
     and "set (xs @ [x]) = set (ys @ [x] @ zs)"
-  shows "crdt_ops deps (ys @ zs @ [x])"
+  shows "crdt_ops (ys @ zs @ [x]) deps"
 using assms proof -
   obtain oid oper where x_pair: "x = (oid, oper)" by force
   hence "\<And>op2 r. op2 \<in> snd ` set zs \<Longrightarrow> r \<in> deps op2 \<Longrightarrow> r \<noteq> oid"
     using assms crdt_ops_independent_suf by fastforce
-  thus "crdt_ops deps (ys @ zs @ [x])"
+  thus "crdt_ops (ys @ zs @ [x]) deps"
     using assms(2) crdt_ops_reorder x_pair by metis
 qed
 
 lemma crdt_ops_rem_spec:
-  assumes "spec_ops deps (xs @ [x])"
-    and "crdt_ops deps (ys @ [x] @ zs)"
+  assumes "spec_ops (xs @ [x]) deps"
+    and "crdt_ops (ys @ [x] @ zs) deps"
     and "set (xs @ [x]) = set (ys @ [x] @ zs)"
-  shows "crdt_ops deps (ys @ zs)"
+  shows "crdt_ops (ys @ zs) deps"
 using assms crdt_ops_rem_last crdt_ops_reorder_spec append_assoc by metis
 
 lemma crdt_ops_rem_penultimate:
-  assumes "crdt_ops deps (xs @ [(i1, r1)] @ [(i2, r2)])"
+  assumes "crdt_ops (xs @ [(i1, r1)] @ [(i2, r2)]) deps"
     and "\<And>r. r \<in> deps r2 \<Longrightarrow> r \<noteq> i1"
-  shows "crdt_ops deps (xs @ [(i2, r2)])"
+  shows "crdt_ops (xs @ [(i2, r2)]) deps"
 proof -
-  have "crdt_ops deps (xs @ [(i1, r1)])"
+  have "crdt_ops (xs @ [(i1, r1)]) deps"
     using assms(1) crdt_ops_rem_last by force
-  hence "crdt_ops deps xs"
+  hence "crdt_ops xs deps"
     using crdt_ops_rem_last by force
   moreover have "distinct (map fst (xs @ [(i1, r1)] @ [(i2, r2)]))"
     using assms(1) crdt_ops_distinct_fst by blast
   hence "i2 \<notin> set (map fst xs)"
     by auto
-  moreover have "crdt_ops deps ((xs @ [(i1, r1)]) @ [(i2, r2)])"
+  moreover have "crdt_ops ((xs @ [(i1, r1)]) @ [(i2, r2)]) deps"
     using assms(1) by auto
   hence "\<And>r. r \<in> deps r2 \<Longrightarrow> r \<in> fst ` set (xs @ [(i1, r1)])"
     using crdt_ops_ref_exists by metis
@@ -727,7 +735,7 @@ proof -
     using assms(2) by auto
   moreover have "\<And>r. r \<in> deps r2 \<Longrightarrow> r < i2"
     using assms(1) crdt_ops_ref_less by fastforce
-  ultimately show "crdt_ops deps (xs @ [(i2, r2)])"
+  ultimately show "crdt_ops (xs @ [(i2, r2)]) deps"
     by (simp add: crdt_ops_intro)
 qed
 
