isabelle/Interleaving.thy
@@ -12,22 +12,22 @@ theory Interleaving
   imports Insert_Spec
 begin
 
-lemma interp_list_maybe_grow:
+lemma interp_ins_maybe_grow:
   assumes "insert_ops (xs @ [(oid, ref)])"
-  shows "set (interp_list (xs @ [(oid, ref)])) = set (interp_list xs) \<or>
-         set (interp_list (xs @ [(oid, ref)])) = (set (interp_list xs) \<union> {oid})"
-by (cases ref, simp add: interp_list_tail_unfold,
-    metis insert_spec_nonex insert_spec_set interp_list_tail_unfold)
+  shows "set (interp_ins (xs @ [(oid, ref)])) = set (interp_ins xs) \<or>
+         set (interp_ins (xs @ [(oid, ref)])) = (set (interp_ins xs) \<union> {oid})"
+by (cases ref, simp add: interp_ins_tail_unfold,
+    metis insert_spec_nonex insert_spec_set interp_ins_tail_unfold)
 
-lemma interp_list_maybe_grow2:
+lemma interp_ins_maybe_grow2:
   assumes "insert_ops (xs @ [x])"
-  shows "set (interp_list (xs @ [x])) = set (interp_list xs) \<or>
-         set (interp_list (xs @ [x])) = (set (interp_list xs) \<union> {fst x})"
-using assms interp_list_maybe_grow by (cases x, auto)
+  shows "set (interp_ins (xs @ [x])) = set (interp_ins xs) \<or>
+         set (interp_ins (xs @ [x])) = (set (interp_ins xs) \<union> {fst x})"
+using assms interp_ins_maybe_grow by (cases x, auto)
 
-lemma interp_list_maybe_grow3:
+lemma interp_ins_maybe_grow3:
   assumes "insert_ops (xs @ ys)"
-  shows "\<exists>A. A \<subseteq> set (map fst ys) \<and> set (interp_list (xs @ ys)) = set (interp_list xs) \<union> A"
+  shows "\<exists>A. A \<subseteq> set (map fst ys) \<and> set (interp_ins (xs @ ys)) = set (interp_ins xs) \<union> A"
 using assms proof(induction ys rule: List.rev_induct)
   case Nil
   then show ?case by simp
@@ -36,10 +36,10 @@ next
   then have "insert_ops (xs @ ys)"
     by (metis append_assoc insert_ops_rem_last)
   then obtain A where IH: "A \<subseteq> set (map fst ys) \<and>
-            set (interp_list (xs @ ys)) = set (interp_list xs) \<union> A"
+            set (interp_ins (xs @ ys)) = set (interp_ins xs) \<union> A"
     using snoc.IH by blast
   then show ?case
-  proof(cases "set (interp_list (xs @ ys @ [x])) = set (interp_list (xs @ ys))")
+  proof(cases "set (interp_ins (xs @ ys @ [x])) = set (interp_ins (xs @ ys))")
     case True
     moreover have "A \<subseteq> set (map fst (ys @ [x]))"
       using IH by auto
@@ -47,8 +47,8 @@ next
       using IH by auto
   next
     case False
-    then have "set (interp_list (xs @ ys @ [x])) = set (interp_list (xs @ ys)) \<union> {fst x}"
-      by (metis append_assoc interp_list_maybe_grow2 snoc.prems)
+    then have "set (interp_ins (xs @ ys @ [x])) = set (interp_ins (xs @ ys)) \<union> {fst x}"
+      by (metis append_assoc interp_ins_maybe_grow2 snoc.prems)
     moreover have "A \<union> {fst x} \<subseteq> set (map fst (ys @ [x]))"
       using IH by auto
     ultimately show ?thesis
@@ -56,26 +56,26 @@ next
   qed
 qed
 
-lemma interp_list_ref_nonex:
+lemma interp_ins_ref_nonex:
   assumes "insert_ops ops"
     and "ops = xs @ [(oid, Some ref)] @ ys"
-    and "ref \<notin> set (interp_list xs)"
-  shows "oid \<notin> set (interp_list ops)"
+    and "ref \<notin> set (interp_ins xs)"
+  shows "oid \<notin> set (interp_ins ops)"
 using assms proof(induction ys arbitrary: ops rule: List.rev_induct)
   case Nil
-  then have "interp_list ops = insert_spec (interp_list xs) (oid, Some ref)"
-    by (simp add: interp_list_tail_unfold)
+  then have "interp_ins ops = insert_spec (interp_ins xs) (oid, Some ref)"
+    by (simp add: interp_ins_tail_unfold)
   moreover have "\<And>i. i \<in> set (map fst xs) \<Longrightarrow> i < oid"
     using Nil.prems last_op_greatest by fastforce
-  hence "\<And>i. i \<in> set (interp_list xs) \<Longrightarrow> i < oid"
-    by (meson interp_list_subset subsetCE)
-  ultimately show "oid \<notin> set (interp_list ops)"
+  hence "\<And>i. i \<in> set (interp_ins xs) \<Longrightarrow> i < oid"
+    by (meson interp_ins_subset subsetCE)
+  ultimately show "oid \<notin> set (interp_ins ops)"
     using assms(3) by auto
 next
   case (snoc x ys)
   then have "insert_ops (xs @ (oid, Some ref) # ys)"
     by (metis append.assoc append.simps(1) append_Cons insert_ops_appendD)
-  hence IH: "oid \<notin> set (interp_list (xs @ (oid, Some ref) # ys))"
+  hence IH: "oid \<notin> set (interp_ins (xs @ (oid, Some ref) # ys))"
     by (simp add: snoc.IH snoc.prems(3))
   moreover have "distinct (map fst (xs @ (oid, Some ref) # ys @ [x]))"
     using snoc.prems by (metis append_Cons append_self_conv2 insert_ops_def spec_ops_def)
@@ -83,12 +83,12 @@ next
     using empty_iff by auto
   moreover have "insert_ops ((xs @ (oid, Some ref) # ys) @ [x])"
     using snoc.prems by auto
-  hence "set (interp_list ((xs @ (oid, Some ref) # ys) @ [x])) =
-         set (interp_list (xs @ (oid, Some ref) # ys)) \<or> 
-         set (interp_list ((xs @ (oid, Some ref) # ys) @ [x])) =
-         set (interp_list (xs @ (oid, Some ref) # ys)) \<union> {fst x}"
-    using interp_list_maybe_grow2 by blast
-  ultimately show "oid \<notin> set (interp_list ops)"
+  hence "set (interp_ins ((xs @ (oid, Some ref) # ys) @ [x])) =
+         set (interp_ins (xs @ (oid, Some ref) # ys)) \<or> 
+         set (interp_ins ((xs @ (oid, Some ref) # ys) @ [x])) =
+         set (interp_ins (xs @ (oid, Some ref) # ys)) \<union> {fst x}"
+    using interp_ins_maybe_grow2 by blast
+  ultimately show "oid \<notin> set (interp_ins ops)"
     using snoc.prems(2) by auto
 qed
 
@@ -226,15 +226,15 @@ proof -
     using xy_split z_split by blast
 qed
 
-lemma interp_list_last_None:
-  shows "oid \<in> set (interp_list (ops @ [(oid, None)]))"
-by (simp add: interp_list_tail_unfold)
+lemma interp_ins_last_None:
+  shows "oid \<in> set (interp_ins (ops @ [(oid, None)]))"
+by (simp add: interp_ins_tail_unfold)
 
-lemma interp_list_monotonic:
+lemma interp_ins_monotonic:
   assumes "insert_ops (pre @ suf)"
-    and "oid \<in> set (interp_list pre)"
-  shows "oid \<in> set (interp_list (pre @ suf))"
-using assms interp_list_maybe_grow3 by auto
+    and "oid \<in> set (interp_ins pre)"
+  shows "oid \<in> set (interp_ins (pre @ suf))"
+using assms interp_ins_maybe_grow3 by auto
 
 lemma insert_ops_sorted_oids:
   assumes "insert_ops (xs @ [(i1, r1)] @ ys @ [(i2, r2)])"
@@ -248,43 +248,43 @@ proof -
     by blast
 qed
 
-lemma interp_list_append_non_memb:
+lemma interp_ins_append_non_memb:
   assumes "insert_ops (pre @ [(oid, Some ref)] @ suf)"
-    and "ref \<notin> set (interp_list pre)"
-  shows "ref \<notin> set (interp_list (pre @ [(oid, Some ref)] @ suf))"
+    and "ref \<notin> set (interp_ins pre)"
+  shows "ref \<notin> set (interp_ins (pre @ [(oid, Some ref)] @ suf))"
 using assms proof(induction suf rule: List.rev_induct)
   case Nil
-  then show "ref \<notin> set (interp_list (pre @ [(oid, Some ref)] @ []))"
-    by (metis append_Nil2 insert_spec_nonex interp_list_tail_unfold)
+  then show "ref \<notin> set (interp_ins (pre @ [(oid, Some ref)] @ []))"
+    by (metis append_Nil2 insert_spec_nonex interp_ins_tail_unfold)
 next
   case (snoc x xs)
-  hence IH: "ref \<notin> set (interp_list (pre @ [(oid, Some ref)] @ xs))"
+  hence IH: "ref \<notin> set (interp_ins (pre @ [(oid, Some ref)] @ xs))"
     by (metis append_assoc insert_ops_rem_last)
   moreover have "ref < oid"
     using insert_ops_ref_older snoc.prems(1) by auto
   moreover have "oid < fst x"
     using insert_ops_sorted_oids by (metis prod.collapse snoc.prems(1))
-  have "set (interp_list ((pre @ [(oid, Some ref)] @ xs) @ [x])) =
-        set (interp_list (pre @ [(oid, Some ref)] @ xs)) \<or>
-        set (interp_list ((pre @ [(oid, Some ref)] @ xs) @ [x])) =
-        set (interp_list (pre @ [(oid, Some ref)] @ xs)) \<union> {fst x}"
-    by (metis (full_types) append.assoc interp_list_maybe_grow2 snoc.prems(1))
-  ultimately show "ref \<notin> set (interp_list (pre @ [(oid, Some ref)] @ xs @ [x]))"
+  have "set (interp_ins ((pre @ [(oid, Some ref)] @ xs) @ [x])) =
+        set (interp_ins (pre @ [(oid, Some ref)] @ xs)) \<or>
+        set (interp_ins ((pre @ [(oid, Some ref)] @ xs) @ [x])) =
+        set (interp_ins (pre @ [(oid, Some ref)] @ xs)) \<union> {fst x}"
+    by (metis (full_types) append.assoc interp_ins_maybe_grow2 snoc.prems(1))
+  ultimately show "ref \<notin> set (interp_ins (pre @ [(oid, Some ref)] @ xs @ [x]))"
     using \<open>oid < fst x\<close> by auto
 qed
 
-lemma interp_list_append_memb:
+lemma interp_ins_append_memb:
   assumes "insert_ops (pre @ [(oid, Some ref)] @ suf)"
-    and "ref \<in> set (interp_list pre)"
-  shows "oid \<in> set (interp_list (pre @ [(oid, Some ref)] @ suf))"
-using assms by (metis UnCI append_assoc insert_spec_set interp_list_monotonic
-  interp_list_tail_unfold singletonI)
+    and "ref \<in> set (interp_ins pre)"
+  shows "oid \<in> set (interp_ins (pre @ [(oid, Some ref)] @ suf))"
+using assms by (metis UnCI append_assoc insert_spec_set interp_ins_monotonic
+  interp_ins_tail_unfold singletonI)
 
-lemma interp_list_append_forward:
+lemma interp_ins_append_forward:
   assumes "insert_ops (xs @ ys)"
-    and "oid \<in> set (interp_list (xs @ ys))"
+    and "oid \<in> set (interp_ins (xs @ ys))"
     and "oid \<in> set (map fst xs)"
-  shows "oid \<in> set (interp_list xs)"
+  shows "oid \<in> set (interp_ins xs)"
 using assms proof(induction ys rule: List.rev_induct, simp)
   case (snoc y ys)
   obtain cs ds ref where "xs = cs @ (oid, ref) # ds"
@@ -297,18 +297,24 @@ using assms proof(induction ys rule: List.rev_induct, simp)
     by blast
   then show ?case
     using snoc.IH snoc.prems(1) snoc.prems(2) assms(3) inserted_item_ident
-    by (metis append_assoc insert_ops_appendD interp_list_tail_unfold prod.collapse)
+    by (metis append_assoc insert_ops_appendD interp_ins_tail_unfold prod.collapse)
 qed
 
-lemma interp_list_find_ref:
+lemma interp_ins_nonex_forward:
+  assumes "insert_ops (xs @ ys)"
+    and "oid \<notin> set (interp_ins (xs @ ys))"
+  shows "oid \<notin> set (interp_ins xs)"
+using assms interp_ins_monotonic by blast
+
+lemma interp_ins_find_ref:
   assumes "insert_ops (xs @ [(oid, Some ref)] @ ys)"
-    and "ref \<in> set (interp_list (xs @ [(oid, Some ref)] @ ys))"
+    and "ref \<in> set (interp_ins (xs @ [(oid, Some ref)] @ ys))"
   shows "\<exists>r. (ref, r) \<in> set xs"
 proof -
   have "ref < oid"
     using assms(1) insert_ops_ref_older by blast
   have "ref \<in> set (map fst (xs @ [(oid, Some ref)] @ ys))"
-    by (meson assms(2) interp_list_subset subsetCE)
+    by (meson assms(2) interp_ins_subset subsetCE)
   then obtain x where x_prop: "x \<in> set (xs @ [(oid, Some ref)] @ ys) \<and> fst x = ref"
     by fastforce
   obtain xr where x_pair: "x = (ref, xr)"
@@ -346,29 +352,29 @@ by (metis Un_iff assms list_order_monotonic insert_ops_appendD set_append subset
 
 lemma list_order_insert_ref:
   assumes "insert_ops (ops @ [(oid, Some ref)])"
-    and "ref \<in> set (interp_list ops)"
+    and "ref \<in> set (interp_ins ops)"
   shows "list_order (ops @ [(oid, Some ref)]) ref oid"
 proof -
-  have "interp_list (ops @ [(oid, Some ref)]) = insert_spec (interp_list ops) (oid, Some ref)"
-    by (simp add: interp_list_tail_unfold)
-  moreover obtain xs ys where "interp_list ops = xs @ [ref] @ ys"
+  have "interp_ins (ops @ [(oid, Some ref)]) = insert_spec (interp_ins ops) (oid, Some ref)"
+    by (simp add: interp_ins_tail_unfold)
+  moreover obtain xs ys where "interp_ins ops = xs @ [ref] @ ys"
     using assms(2) split_list_first by fastforce
-  hence "insert_spec (interp_list ops) (oid, Some ref) = xs @ [ref] @ [] @ [oid] @ ys"
-    using assms(1) insert_after_ref interp_list_distinct by fastforce
+  hence "insert_spec (interp_ins ops) (oid, Some ref) = xs @ [ref] @ [] @ [oid] @ ys"
+    using assms(1) insert_after_ref interp_ins_distinct by fastforce
   ultimately show "list_order (ops @ [(oid, Some ref)]) ref oid"
     using assms(1) list_orderI by metis
 qed
 
 lemma list_order_insert_none:
   assumes "insert_ops (ops @ [(oid, None)])"
-    and "x \<in> set (interp_list ops)"
+    and "x \<in> set (interp_ins ops)"
   shows "list_order (ops @ [(oid, None)]) oid x"
 proof -
-  have "interp_list (ops @ [(oid, None)]) = insert_spec (interp_list ops) (oid, None)"
-    by (simp add: interp_list_tail_unfold)
-  moreover obtain xs ys where "interp_list ops = xs @ [x] @ ys"
+  have "interp_ins (ops @ [(oid, None)]) = insert_spec (interp_ins ops) (oid, None)"
+    by (simp add: interp_ins_tail_unfold)
+  moreover obtain xs ys where "interp_ins ops = xs @ [x] @ ys"
     using assms(2) split_list_first by fastforce
-  hence "insert_spec (interp_list ops) (oid, None) = [] @ [oid] @ xs @ [x] @ ys"
+  hence "insert_spec (interp_ins ops) (oid, None) = [] @ [oid] @ xs @ [x] @ ys"
     by simp
   ultimately show "list_order (ops @ [(oid, None)]) oid x"
     using assms(1) list_orderI by metis
@@ -379,14 +385,14 @@ lemma list_order_insert_between:
     and "list_order ops ref x"
   shows "list_order (ops @ [(oid, Some ref)]) oid x"
 proof -
-  have "interp_list (ops @ [(oid, Some ref)]) = insert_spec (interp_list ops) (oid, Some ref)"
-    by (simp add: interp_list_tail_unfold)
-  moreover obtain xs ys zs where "interp_list ops = xs @ [ref] @ ys @ [x] @ zs"
+  have "interp_ins (ops @ [(oid, Some ref)]) = insert_spec (interp_ins ops) (oid, Some ref)"
+    by (simp add: interp_ins_tail_unfold)
+  moreover obtain xs ys zs where "interp_ins ops = xs @ [ref] @ ys @ [x] @ zs"
     using assms list_orderE by blast
   moreover have "... = xs @ ref # (ys @ [x] @ zs)"
     by simp
   moreover have "distinct (xs @ ref # (ys @ [x] @ zs))"
-    using assms(1) calculation by (metis interp_list_distinct insert_ops_rem_last)
+    using assms(1) calculation by (metis interp_ins_distinct insert_ops_rem_last)
   hence "insert_spec (xs @ ref # (ys @ [x] @ zs)) (oid, Some ref) = xs @ ref # oid # (ys @ [x] @ zs)"
     using assms(1) calculation by (simp add: insert_after_ref)
   moreover have "... = (xs @ [ref]) @ [oid] @ ys @ [x] @ zs"
@@ -441,16 +447,16 @@ lemma insert_seq_ref_missing:
     and "insert_ops ops" and "insert_ops xs"
     and "set xs \<subseteq> set ops"
     and "ops = as @ [hd xs] @ bs"
-    and "r \<notin> set (interp_list as)"
-  shows "\<forall>x \<in> set (map fst xs). x \<notin> set (interp_list ops)"
+    and "r \<notin> set (interp_ins as)"
+  shows "\<forall>x \<in> set (map fst xs). x \<notin> set (interp_ins ops)"
 using assms proof(induction xs rule: List.rev_induct, simp)
   case snoc_x: (snoc x xs)
-  then show "\<forall>x \<in> set (map fst (xs @ [x])). x \<notin> set (interp_list ops)"
+  then show "\<forall>x \<in> set (map fst (xs @ [x])). x \<notin> set (interp_ins ops)"
   proof(cases "xs = []")
     case True
-    moreover from this have "fst x \<notin> set (interp_list ops)"
-      using interp_list_ref_nonex insert_seq_hd snoc_x.prems by fastforce
-    ultimately show "\<forall>x \<in> set (map fst (xs @ [x])). x \<notin> set (interp_list ops)"
+    moreover from this have "fst x \<notin> set (interp_ins ops)"
+      using interp_ins_ref_nonex insert_seq_hd snoc_x.prems by fastforce
+    ultimately show "\<forall>x \<in> set (map fst (xs @ [x])). x \<notin> set (interp_ins ops)"
       by auto 
   next
     case xs_nonempty: False
@@ -460,7 +466,7 @@ using assms proof(induction xs rule: List.rev_induct, simp)
       by force
     then have "xr = Some yi"
       using insert_seq_last_ref snoc_x.prems(1) snoc_y by force
-    have IH: "\<forall>x \<in> set (map fst xs). x \<notin> set (interp_list ops)"
+    have IH: "\<forall>x \<in> set (map fst xs). x \<notin> set (interp_ins ops)"
     proof -
       have "insert_seq (Some r) xs"
         using snoc_x.prems(1) insert_seq_rem_last xs_nonempty by blast
@@ -475,16 +481,16 @@ using assms proof(induction xs rule: List.rev_induct, simp)
       using snoc_x.prems(4) by auto
     then obtain as bs where "ops = as @ x # bs"
       by (meson split_list)
-    have "yi \<notin> set (interp_list ops)"
+    have "yi \<notin> set (interp_ins ops)"
       using IH by (simp add: yx_pairs snoc_y)
-    hence "yi \<notin> set (interp_list as)"
-      using \<open>ops = as @ x # bs\<close> interp_list_monotonic snoc_x.prems(2) by blast
-    hence "xi \<notin> set (interp_list ops)"
-      using interp_list_ref_nonex \<open>ops = as @ x # bs\<close> \<open>xr = Some yi\<close>
+    hence "yi \<notin> set (interp_ins as)"
+      using \<open>ops = as @ x # bs\<close> interp_ins_monotonic snoc_x.prems(2) by blast
+    hence "xi \<notin> set (interp_ins ops)"
+      using interp_ins_ref_nonex \<open>ops = as @ x # bs\<close> \<open>xr = Some yi\<close>
         append.simps(2) snoc_x.prems(2) yx_pairs by fastforce
     moreover have "set (map fst (xs @ [x])) = set (map fst xs) \<union> {xi}"
       using yx_pairs by auto
-    ultimately show "\<forall>x \<in> set (map fst (xs @ [x])). x \<notin> set (interp_list ops)"
+    ultimately show "\<forall>x \<in> set (map fst (xs @ [x])). x \<notin> set (interp_ins ops)"
       by simp
   qed
 qed
@@ -493,7 +499,7 @@ qed
   assumes "insert_ops (ops @ [(oid, start)])"
     and "insert_seq start xs" and "insert_ops xs"
     and "set xs \<subseteq> set ops"
-    and "start = None \<or> (\<exists>r. start = Some r \<and> r \<in> set (interp_list ops))"
+    and "start = None \<or> (\<exists>r. start = Some r \<and> r \<in> set (interp_ins ops))"
   shows "\<forall>x \<in> set (map fst xs). list_order (ops @ [(oid, start)]) oid x"
 using assms proof(induction xs rule: List.rev_induct, simp)
   case (snoc x xs)
@@ -507,15 +513,15 @@ using assms proof(induction xs rule: List.rev_induct, simp)
     case True
     then have "snd x = start"
       using snoc.prems(2) insert_seq_hd by fastforce
-    hence "fst x \<in> set (interp_list ops)"
+    hence "fst x \<in> set (interp_ins ops)"
     proof(cases start)
       case None
-      hence "fst x \<in> set (interp_list (as @ [x]))"
-        by (metis \<open>snd x = start\<close> interp_list_last_None prod.collapse)
+      hence "fst x \<in> set (interp_ins (as @ [x]))"
+        by (metis \<open>snd x = start\<close> interp_ins_last_None prod.collapse)
       moreover have "ops = (as @ [x]) @ bs"
         using x_split by simp
       ultimately show ?thesis
-        using snoc.prems(1) interp_list_monotonic by blast
+        using snoc.prems(1) interp_ins_monotonic by blast
     next
       case (Some a)
       then show ?thesis sorry
@@ -534,13 +540,13 @@ lemma insert_seq_start_none:
   assumes "insert_ops ops"
     and "insert_seq None xs" and "insert_ops xs"
     and "set xs \<subseteq> set ops"
-  shows "\<forall>i \<in> set (map fst xs). i \<in> set (interp_list ops)"
+  shows "\<forall>i \<in> set (map fst xs). i \<in> set (interp_ins ops)"
 using assms proof(induction xs rule: List.rev_induct, simp)
   case (snoc x xs)
-  then have IH: "\<forall>i \<in> set (map fst xs). i \<in> set (interp_list ops)"
+  then have IH: "\<forall>i \<in> set (map fst xs). i \<in> set (interp_ins ops)"
     by (metis Nil_is_map_conv append_is_Nil_conv insert_ops_appendD insert_seq_rem_last
         le_supE list.simps(3) set_append split_list)
-  then show "\<forall>i \<in> set (map fst (xs @ [x])). i \<in> set (interp_list ops)"
+  then show "\<forall>i \<in> set (map fst (xs @ [x])). i \<in> set (interp_ins ops)"
   proof(cases "xs = []")
     case True
     then obtain oid where "xs @ [x] = [(oid, None)]"
@@ -551,11 +557,11 @@ using assms proof(induction xs rule: List.rev_induct, simp)
       by (meson split_list)
     hence "ops = (as @ [(oid, None)]) @ bs"
       by (simp add: \<open>ops = as @ (oid, None) # bs\<close>)
-    moreover have "oid \<in> set (interp_list (as @ [(oid, None)]))"
-      by (simp add: interp_list_last_None)
-    ultimately have "oid \<in> set (interp_list ops)"
-      using interp_list_monotonic snoc.prems(1) by blast
-    then show "\<forall>i \<in> set (map fst (xs @ [x])). i \<in> set (interp_list ops)" 
+    moreover have "oid \<in> set (interp_ins (as @ [(oid, None)]))"
+      by (simp add: interp_ins_last_None)
+    ultimately have "oid \<in> set (interp_ins ops)"
+      using interp_ins_monotonic snoc.prems(1) by blast
+    then show "\<forall>i \<in> set (map fst (xs @ [x])). i \<in> set (interp_ins ops)" 
       using \<open>xs @ [x] = [(oid, None)]\<close> by auto
   next
     case False
@@ -572,22 +578,22 @@ using assms proof(induction xs rule: List.rev_induct, simp)
       using snoc.prems(4) snoc_y yx_pairs \<open>xr = Some yi\<close> by auto
     then obtain as bs cs where ops_split: "ops = as @ [(yi, yr)] @ bs @ [(xi, Some yi)] @ cs"
       using insert_ops_split_2 \<open>yi < xi\<close> snoc.prems(1) by blast
-    hence "yi \<in> set (interp_list (as @ [(yi, yr)] @ bs))"
+    hence "yi \<in> set (interp_ins (as @ [(yi, yr)] @ bs))"
     proof -
-      have "yi \<in> set (interp_list ops)"
+      have "yi \<in> set (interp_ins ops)"
         by (simp add: IH snoc_y yx_pairs)
       moreover have "ops = (as @ [(yi, yr)] @ bs) @ ([(xi, Some yi)] @ cs)"
         using ops_split by simp
       moreover have "yi \<in> set (map fst (as @ [(yi, yr)] @ bs))"
         by simp
       ultimately show ?thesis
-        using snoc.prems(1) interp_list_append_forward by blast
+        using snoc.prems(1) interp_ins_append_forward by blast
     qed
-    hence "xi \<in> set (interp_list ((as @ [(yi, yr)] @ bs) @ [(xi, Some yi)] @ cs))"
-      using snoc.prems(1) interp_list_append_memb ops_split by force
-    hence "xi \<in> set (interp_list ops)"
+    hence "xi \<in> set (interp_ins ((as @ [(yi, yr)] @ bs) @ [(xi, Some yi)] @ cs))"
+      using snoc.prems(1) interp_ins_append_memb ops_split by force
+    hence "xi \<in> set (interp_ins ops)"
       by (simp add: ops_split)
-    then show "\<forall>i \<in> set (map fst (xs @ [x])). i \<in> set (interp_list ops)"
+    then show "\<forall>i \<in> set (map fst (xs @ [x])). i \<in> set (interp_ins ops)"
       using IH yx_pairs by auto
   qed
 qed
@@ -596,7 +602,7 @@ lemma insert_seq_after_start:
   assumes "insert_ops ops"
     and "insert_seq (Some ref) xs" and "insert_ops xs"
     and "set xs \<subseteq> set ops"
-    and "ref \<in> set (interp_list ops)"
+    and "ref \<in> set (interp_ins ops)"
   shows "\<forall>i \<in> set (map fst xs). list_order ops ref i"
 using assms proof(induction xs rule: List.rev_induct, simp)
   case (snoc x xs)
@@ -618,14 +624,14 @@ using assms proof(induction xs rule: List.rev_induct, simp)
         using x_split \<open>snd x = Some ref\<close>
         by (metis append_Cons append_self_conv2 prod.collapse snoc.prems(1))
       moreover from this obtain rr where "(ref, rr) \<in> set cs"
-        using interp_list_find_ref x_split \<open>snd x = Some ref\<close> assms(5)
+        using interp_ins_find_ref x_split \<open>snd x = Some ref\<close> assms(5)
         by (metis (no_types, lifting) append_Cons append_self_conv2 prod.collapse)
-      hence "ref \<in> set (interp_list cs)"
+      hence "ref \<in> set (interp_ins cs)"
       proof -
         have "ops = cs @ ([(fst x, Some ref)] @ ds)"
           by (metis x_split \<open>snd x = Some ref\<close> append_Cons append_self_conv2 prod.collapse)
-        thus "ref \<in> set (interp_list cs)"
-          using assms(5) calculation interp_list_append_forward interp_list_append_non_memb by blast
+        thus "ref \<in> set (interp_ins cs)"
+          using assms(5) calculation interp_ins_append_forward interp_ins_append_non_memb by blast
       qed
       ultimately show "list_order (cs @ [(fst x, Some ref)]) ref (fst x)"
         using list_order_insert_ref by (metis append.assoc insert_ops_appendD)
@@ -658,10 +664,10 @@ using assms proof(induction xs rule: List.rev_induct, simp)
         using ops_split snoc.prems(1) by auto
       hence "insert_ops ((as @ [(yi, yr)] @ bs) @ [(xi, Some yi)])"
         using insert_ops_appendD by fastforce
-      moreover have "yi \<in> set (interp_list ops)"
+      moreover have "yi \<in> set (interp_ins ops)"
         using \<open>list_order ops ref yi\<close> list_order_memb2 by auto
-      hence "yi \<in> set (interp_list (as @ [(yi, yr)] @ bs))"
-        using interp_list_append_non_memb ops_split snoc.prems(1) by force
+      hence "yi \<in> set (interp_ins (as @ [(yi, yr)] @ bs))"
+        using interp_ins_append_non_memb ops_split snoc.prems(1) by force
       ultimately show ?thesis
         using list_order_insert_ref by force
     qed
@@ -674,22 +680,22 @@ using assms proof(induction xs rule: List.rev_induct, simp)
     by auto
 qed
 
-lemma insert_seq_no_start:
+(*lemma insert_seq_no_start:
   assumes "insert_ops ops"
     and "insert_seq (Some ref) xs" and "insert_ops xs"
     and "set xs \<subseteq> set ops"
-    and "ref \<notin> set (interp_list ops)"
-  shows "\<forall>i \<in> set (map fst xs). i \<notin> set (interp_list ops)"
+    and "ref \<notin> set (interp_ins ops)"
+  shows "\<forall>i \<in> set (map fst xs). i \<notin> set (interp_ins ops)"
 using assms proof(induction xs rule: List.rev_induct, simp)
   case (snoc x xs)
-  have IH: "\<forall>i \<in> set (map fst xs). i \<notin> set (interp_list ops)"
+  have IH: "\<forall>i \<in> set (map fst xs). i \<notin> set (interp_ins ops)"
     using snoc.IH snoc.prems insert_seq_rem_last insert_ops_appendD
     by (metis append_is_Nil_conv le_sup_iff list.map_disc_iff set_append split_list_first)
-  moreover have "fst x \<notin> set (interp_list ops)"
+  moreover have "fst x \<notin> set (interp_ins ops)"
     sorry
-  ultimately show "\<forall>i \<in> set (map fst (xs @ [x])). i \<notin> set (interp_list ops)"
+  ultimately show "\<forall>i \<in> set (map fst (xs @ [x])). i \<notin> set (interp_ins ops)"
     by auto
-qed
+qed*)
 
 
 (*lemma insert_seq_after_start:
@@ -697,14 +703,14 @@ qed
     and "insert_seq (Some ref) xs" and "insert_ops xs"
     and "set xs \<subseteq> set ops"
   shows "(\<forall>i \<in> set (map fst xs). list_order ops ref i) \<or>
-         (\<forall>i \<in> set (map fst xs). i \<notin> set (interp_list ops))"
+         (\<forall>i \<in> set (map fst xs). i \<notin> set (interp_ins ops))"
 proof -
   have "hd xs \<in> set ops"
     using assms(2) assms(4) hd_in_set insert_seq_nonempty by blast
   then obtain as bs where "ops = as @ (hd xs) # bs"
     by (meson split_list)
   show ?thesis
-  proof(cases "ref \<in> set (interp_list ops)")
+  proof(cases "ref \<in> set (interp_ins ops)")
     case ref_exist: True
     have "\<forall>i \<in> set (map fst xs). list_order ops ref i"
       using assms proof(induction xs rule: List.rev_induct, simp)
@@ -724,11 +730,11 @@ proof -
         hence "insert_ops (cs @ [(fst x, Some ref)] @ ds)"
           by (metis \<open>snd x = Some ref\<close> append_Cons append_self_conv2 prod.collapse snoc.prems(1))
         then obtain rr where "(ref, rr) \<in> set cs"
-          using interp_list_find_ref \<open>ops = cs @ x # ds\<close> \<open>snd x = Some ref\<close> ref_exist
+          using interp_ins_find_ref \<open>ops = cs @ x # ds\<close> \<open>snd x = Some ref\<close> ref_exist
           by (metis (no_types, lifting) append_Cons append_self_conv2 prod.collapse)
-        hence "ref \<in> set (interp_list cs)"
-          (* why not use interp_list_append_forward? *)
-          using interp_list_append_non_memb \<open>ops = cs @ x # ds\<close> \<open>snd x = Some ref\<close>
+        hence "ref \<in> set (interp_ins cs)"
+          (* why not use interp_ins_append_forward? *)
+          using interp_ins_append_non_memb \<open>ops = cs @ x # ds\<close> \<open>snd x = Some ref\<close>
           by (metis append_Cons prod.collapse ref_exist self_append_conv2 snoc.prems(1))
         hence "list_order (cs @ [(fst x, Some ref)]) ref (fst x)"
           using list_order_insert_ref \<open>insert_ops (cs @ [(fst x, Some ref)] @ ds)\<close>
@@ -747,15 +753,15 @@ proof -
     then show ?thesis by blast
   next
     case ref_nexist: False
-    have "\<forall>i \<in> set (map fst xs). i \<notin> set (interp_list ops)"
+    have "\<forall>i \<in> set (map fst xs). i \<notin> set (interp_ins ops)"
       using assms proof(induction xs rule: List.rev_induct, simp)
       case (snoc x xs)
-      have IH: "\<forall>i \<in> set (map fst xs). i \<notin> set (interp_list ops)"
+      have IH: "\<forall>i \<in> set (map fst xs). i \<notin> set (interp_ins ops)"
         using snoc.IH snoc.prems insert_seq_rem_last insert_ops_appendD
         by (metis append_is_Nil_conv le_sup_iff list.map_disc_iff set_append split_list_first)
-      moreover have "fst x \<notin> set (interp_list ops)"
+      moreover have "fst x \<notin> set (interp_ins ops)"
         sorry
-      ultimately show "\<forall>i \<in> set (map fst (xs @ [x])). i \<notin> set (interp_list ops)"
+      ultimately show "\<forall>i \<in> set (map fst (xs @ [x])). i \<notin> set (interp_ins ops)"
         by auto
     qed
     then show ?thesis by blast
@@ -851,7 +857,7 @@ next
     using Cons.IH Cons.prems by auto
 qed
 
-theorem no_interleaving_general:
+(*theorem no_interleaving_general:
   assumes "insert_ops ops"
     and "insert_seq start xs" and "insert_ops xs"
     and "insert_seq start ys" and "insert_ops ys"
@@ -861,7 +867,7 @@ theorem no_interleaving_general:
            (\<forall>x \<in> set (map fst xs). \<forall>y \<in> set (map fst ys). list_order ops y x)) \<and>
           (\<forall>r. start = Some r \<longrightarrow> (\<forall>x \<in> set (map fst xs). list_order ops r x) \<and>
                                   (\<forall>y \<in> set (map fst ys). list_order ops r y))) \<or>
-         (\<forall>x \<in> set (map fst xs) \<union> set (map fst ys). x \<notin> set (interp_list ops))"
+         (\<forall>x \<in> set (map fst xs) \<union> set (map fst ys). x \<notin> set (interp_ins ops))"
 using assms proof(induction ops arbitrary: xs ys rule: List.rev_induct, simp)
   case (snoc a ops)
   then have "insert_ops ops"
@@ -881,11 +887,11 @@ using assms proof(induction ops arbitrary: xs ys rule: List.rev_induct, simp)
                 (\<forall>x \<in> set (map fst (butlast xs)). \<forall>y \<in> set (map fst ys). list_order ops y x)) \<and>
                (\<forall>r. start = Some r \<longrightarrow> (\<forall>x \<in> set (map fst (butlast xs)). list_order ops r x) \<and>
                                        (\<forall>y \<in> set (map fst ys).           list_order ops r y))) \<or>
-              (\<forall>x \<in> set (map fst (butlast xs)) \<union> set (map fst ys). x \<notin> set (interp_list ops))"
+              (\<forall>x \<in> set (map fst (butlast xs)) \<union> set (map fst ys). x \<notin> set (interp_ins ops))"
     proof(cases "xs = [a]")
       case True
       moreover have "(\<forall>r. start = Some r \<longrightarrow> (\<forall>y \<in> set (map fst ys). list_order ops r y)) \<or>
-            (\<forall>y \<in> set (map fst ys). y \<notin> set (interp_list ops))"
+            (\<forall>y \<in> set (map fst ys). y \<notin> set (interp_ins ops))"
         using insert_seq_after_start insert_seq_no_start \<open>insert_ops ops\<close> \<open>set ys \<subseteq> set ops\<close>
           snoc.prems(4) snoc.prems(5) by blast
       ultimately show ?thesis by auto
@@ -912,12 +918,12 @@ using assms proof(induction ops arbitrary: xs ys rule: List.rev_induct, simp)
       (y_first) "(\<forall>x \<in> set (map fst (butlast xs)). \<forall>y \<in> set (map fst ys). list_order ops y x) \<and>
                  (\<forall>r. start = Some r \<longrightarrow> (\<forall>x \<in> set (map fst (butlast xs)). list_order ops r x) \<and>
                                          (\<forall>y \<in> set (map fst ys).           list_order ops r y))" |
-      (neither) "\<forall>x \<in> set (map fst (butlast xs)) \<union> set (map fst ys). x \<notin> set (interp_list ops)"
+      (neither) "\<forall>x \<in> set (map fst (butlast xs)) \<union> set (map fst ys). x \<notin> set (interp_ins ops)"
       using IH by blast
     then show ?thesis
     proof(cases)
       case x_first
-      moreover have y_exists: "\<forall>y \<in> set (map fst ys). y \<in> set (interp_list ops)"
+      moreover have y_exists: "\<forall>y \<in> set (map fst ys). y \<in> set (interp_ins ops)"
       proof(cases start)
         case None
         then show ?thesis
@@ -965,8 +971,8 @@ using assms proof(induction ops arbitrary: xs ys rule: List.rev_induct, simp)
       moreover have "\<forall>r. start = Some r \<longrightarrow> list_order (ops @ [a]) r (fst a)"
       proof(cases start, simp)
         case (Some r)
-        moreover have "r \<in> set (interp_list (ops @ [a]))"
-          using list_order_memb1 x_first snoc.prems(1) snoc.prems(4) interp_list_monotonic
+        moreover have "r \<in> set (interp_ins (ops @ [a]))"
+          using list_order_memb1 x_first snoc.prems(1) snoc.prems(4) interp_ins_monotonic
           by (metis calculation insert_seq_nonempty last_in_set list.map_disc_iff)
         ultimately show ?thesis
           using snoc.prems by (simp add: insert_seq_after_start \<open>a = last xs\<close> map_fst_xs)
@@ -978,7 +984,7 @@ using assms proof(induction ops arbitrary: xs ys rule: List.rev_induct, simp)
       then show ?thesis by blast
     next
       case y_first
-      moreover have y_exists: "\<forall>y \<in> set (map fst ys). y \<in> set (interp_list ops)"
+      moreover have y_exists: "\<forall>y \<in> set (map fst ys). y \<in> set (interp_ins ops)"
       proof(cases start)
         case None
         then show ?thesis
@@ -1020,8 +1026,8 @@ using assms proof(induction ops arbitrary: xs ys rule: List.rev_induct, simp)
       moreover have "\<forall>r. start = Some r \<longrightarrow> list_order (ops @ [a]) r (fst a)"
       proof(cases start, simp)
         case (Some r)
-        moreover have "r \<in> set (interp_list (ops @ [a]))"
-          using list_order_memb1 y_first snoc.prems(1) snoc.prems(4) interp_list_monotonic
+        moreover have "r \<in> set (interp_ins (ops @ [a]))"
+          using list_order_memb1 y_first snoc.prems(1) snoc.prems(4) interp_ins_monotonic
           by (metis calculation insert_seq_nonempty last_in_set list.map_disc_iff)
         ultimately show ?thesis
           using snoc.prems by (simp add: insert_seq_after_start \<open>a = last xs\<close> map_fst_xs)
@@ -1033,7 +1039,7 @@ using assms proof(induction ops arbitrary: xs ys rule: List.rev_induct, simp)
       then show ?thesis by blast
     next
       case neither
-      have "\<forall>x \<in> set (map fst xs) \<union> set (map fst ys). x \<notin> set (interp_list (ops @ [a]))"
+      have "\<forall>x \<in> set (map fst xs) \<union> set (map fst ys). x \<notin> set (interp_ins (ops @ [a]))"
         sorry
       then show ?thesis sorry
     qed
@@ -1047,7 +1053,7 @@ using assms proof(induction ops arbitrary: xs ys rule: List.rev_induct, simp)
       using insert_ops_subset_last snoc.prems by blast
     have IH: "(\<forall>x \<in> set (map fst xs). \<forall>y \<in> set (map fst (butlast ys)). list_order ops x y) \<or>
               (\<forall>x \<in> set (map fst xs). \<forall>y \<in> set (map fst (butlast ys)). list_order ops y x) \<or>
-              (\<forall>x \<in> set (map fst xs) \<union> set (map fst (butlast ys)). x \<notin> set (interp_list ops))"
+              (\<forall>x \<in> set (map fst xs) \<union> set (map fst (butlast ys)). x \<notin> set (interp_ins ops))"
     proof(cases "ys = [a]")
       case True
       then show ?thesis by simp
@@ -1074,7 +1080,7 @@ using assms proof(induction ops arbitrary: xs ys rule: List.rev_induct, simp)
     case neither
     then show ?thesis sorry
   qed
-qed
+qed*)
 (*
   obtain x1 y1 where x1_def: "(x1, start) = hd xs" and y1_def: "(y1, start) = hd ys"
     by (metis insert_seq_hd snoc.prems(2) snoc.prems(4))
@@ -1105,15 +1111,15 @@ qed
         by (simp add: \<open>x1 \<noteq> y1\<close> a_pair is_y1)
       then obtain as bs where "ops = as @ [(x1, start)] @ bs"
         using insert_ops_split snoc.prems(1) by blast
-      consider (ref_missing) "\<exists>r. start = Some r \<and> r \<notin> set (interp_list as)"
-        | (ref_exists) "start = None \<or> (\<exists>r. start = Some r \<and> r \<in> set (interp_list as))"
+      consider (ref_missing) "\<exists>r. start = Some r \<and> r \<notin> set (interp_ins as)"
+        | (ref_exists) "start = None \<or> (\<exists>r. start = Some r \<and> r \<in> set (interp_ins as))"
         by fastforce
       then show ?thesis
       proof(cases)
         case ref_missing
         then obtain r where "start = Some r"
           by force
-        then have "\<forall>x \<in> set (map fst xs). x \<notin> set (interp_list ops)"
+        then have "\<forall>x \<in> set (map fst xs). x \<notin> set (interp_ins ops)"
         proof -
           have "insert_seq (Some r) xs"
             using snoc.prems(2) \<open>start = Some r\<close> by blast
@@ -1121,7 +1127,7 @@ qed
             by (simp add: snoc.prems(3))
           moreover have "ops = as @ [hd xs] @ bs"
             by (simp add: \<open>ops = as @ [(x1, start)] @ bs\<close> x1_def)
-          moreover have "r \<notin> set (interp_list as)"
+          moreover have "r \<notin> set (interp_ins as)"
             using \<open>start = Some r\<close> ref_missing by blast
           ultimately show ?thesis
             using insert_seq_ref_missing sorry
@@ -1166,8 +1172,8 @@ theorem no_interleaving:
     and "xid \<noteq> yid" and "yid \<noteq> zid" and "zid \<noteq> xid"
   shows "(list_order ops xid yid \<and> list_order ops yid zid) \<or>
          (list_order ops zid xid \<and> list_order ops xid yid) \<or>
-         (xid \<notin> set (interp_list ops) \<and> yid \<notin> set (interp_list ops) \<and>
-          zid \<notin> set (interp_list ops))"
+         (xid \<notin> set (interp_ins ops) \<and> yid \<notin> set (interp_ins ops) \<and>
+          zid \<notin> set (interp_ins ops))"
 proof(cases "xid < zid")
   case True
   then show ?thesis
@@ -1181,16 +1187,16 @@ proof(cases "xid < zid")
     then show ?thesis
     proof(cases ref)
       case None
-      hence "xid \<in> set (interp_list (as @ [(xid, ref)]))"
-        using interp_list_last_None assms(1) split by metis
-      hence xid_in: "xid \<in> set (interp_list (as @ [(xid, ref)] @ bs))"
-        using interp_list_monotonic assms(1) insert_ops_appendD split append.assoc by metis
+      hence "xid \<in> set (interp_ins (as @ [(xid, ref)]))"
+        using interp_ins_last_None assms(1) split by metis
+      hence xid_in: "xid \<in> set (interp_ins (as @ [(xid, ref)] @ bs))"
+        using interp_ins_monotonic assms(1) insert_ops_appendD split append.assoc by metis
       hence "list_order (as @ [(xid, ref)] @ bs @ [(yid, Some xid)]) xid yid"
         using list_order_insert_ref assms(1) insert_ops_appendD split append.assoc by metis
       hence "list_order ops xid yid"
         using list_order_append assms(1) split append.assoc by metis
-      moreover have "xid \<in> set (interp_list (as @ [(xid, ref)] @ bs @ [(yid, Some xid)] @ cs))"
-        using interp_list_monotonic xid_in assms(1) insert_ops_appendD split append.assoc by metis
+      moreover have "xid \<in> set (interp_ins (as @ [(xid, ref)] @ bs @ [(yid, Some xid)] @ cs))"
+        using interp_ins_monotonic xid_in assms(1) insert_ops_appendD split append.assoc by metis
       hence "list_order (as @ [(xid, ref)] @ bs @ [(yid, Some xid)] @ cs @ [(zid, ref)]) zid xid"
         using list_order_insert_none assms(1) insert_ops_appendD split append.assoc None by metis
       hence "list_order ops zid xid"
@@ -1199,14 +1205,14 @@ proof(cases "xid < zid")
     next
       case (Some r)
       then show ?thesis
-      proof(cases "r \<in> set (interp_list as)")
+      proof(cases "r \<in> set (interp_ins as)")
         case True
         hence r_xid: "list_order (as @ [(xid, ref)]) r xid"
           using list_order_insert_ref assms(1) insert_ops_appendD split append.assoc Some by metis
-        hence "xid \<in> set (interp_list (as @ [(xid, ref)]))"
+        hence "xid \<in> set (interp_ins (as @ [(xid, ref)]))"
           using list_order_memb2 assms(1) split by metis
-        hence xid_in: "xid \<in> set (interp_list (as @ [(xid, ref)] @ bs))"
-          using interp_list_monotonic assms(1) insert_ops_appendD split append.assoc by metis
+        hence xid_in: "xid \<in> set (interp_ins (as @ [(xid, ref)] @ bs))"
+          using interp_ins_monotonic assms(1) insert_ops_appendD split append.assoc by metis
         hence "list_order (as @ [(xid, ref)] @ bs @ [(yid, Some xid)]) xid yid"
           using list_order_insert_ref assms(1) insert_ops_appendD split append.assoc by metis
         hence "list_order ops xid yid"
@@ -1220,16 +1226,16 @@ proof(cases "xid < zid")
         ultimately show ?thesis by blast
       next
         case False
-        hence "xid \<notin> set (interp_list ops)"
-          using interp_list_ref_nonex assms(1) split Some by metis
-        moreover have "xid \<notin> set (interp_list (as @ [(xid, ref)] @ bs))"
-          using interp_list_ref_nonex assms(1) insert_ops_appendD split append.assoc Some False by metis
-        hence "yid \<notin> set (interp_list ops)"
-          using interp_list_ref_nonex assms(1) split append.assoc by metis
-        moreover have "r \<notin> set (interp_list (as @ [(xid, ref)] @ bs @ [(yid, Some xid)] @ cs))"
-          using interp_list_append_non_memb assms(1) insert_ops_appendD split append.assoc Some False by metis
-        hence "zid \<notin> set (interp_list ops)"
-          using interp_list_ref_nonex assms(1) split append.assoc Some by metis
+        hence "xid \<notin> set (interp_ins ops)"
+          using interp_ins_ref_nonex assms(1) split Some by metis
+        moreover have "xid \<notin> set (interp_ins (as @ [(xid, ref)] @ bs))"
+          using interp_ins_ref_nonex assms(1) insert_ops_appendD split append.assoc Some False by metis
+        hence "yid \<notin> set (interp_ins ops)"
+          using interp_ins_ref_nonex assms(1) split append.assoc by metis
+        moreover have "r \<notin> set (interp_ins (as @ [(xid, ref)] @ bs @ [(yid, Some xid)] @ cs))"
+          using interp_ins_append_non_memb assms(1) insert_ops_appendD split append.assoc Some False by metis
+        hence "zid \<notin> set (interp_ins ops)"
+          using interp_ins_ref_nonex assms(1) split append.assoc Some by metis
         ultimately show ?thesis by blast
       qed
     qed
@@ -1243,16 +1249,16 @@ proof(cases "xid < zid")
     then show ?thesis
     proof(cases ref)
       case None
-      hence "xid \<in> set (interp_list (as @ [(xid, ref)]))"
-        using interp_list_last_None assms(1) split by metis
-      hence xid_in: "xid \<in> set (interp_list (as @ [(xid, ref)] @ bs))"
-        using interp_list_monotonic assms(1) insert_ops_appendD split append.assoc by metis
+      hence "xid \<in> set (interp_ins (as @ [(xid, ref)]))"
+        using interp_ins_last_None assms(1) split by metis
+      hence xid_in: "xid \<in> set (interp_ins (as @ [(xid, ref)] @ bs))"
+        using interp_ins_monotonic assms(1) insert_ops_appendD split append.assoc by metis
       hence "list_order (as @ [(xid, ref)] @ bs @ [(zid, ref)]) zid xid"
         using list_order_insert_none assms(1) insert_ops_appendD split append.assoc None by metis
       hence "list_order ops zid xid"
         using list_order_append assms(1) split append.assoc by metis
-      moreover have "xid \<in> set (interp_list (as @ [(xid, ref)] @ bs @ [(zid, ref)] @ cs))"
-        using interp_list_monotonic xid_in assms(1) insert_ops_appendD split append.assoc by metis
+      moreover have "xid \<in> set (interp_ins (as @ [(xid, ref)] @ bs @ [(zid, ref)] @ cs))"
+        using interp_ins_monotonic xid_in assms(1) insert_ops_appendD split append.assoc by metis
       hence "list_order (as @ [(xid, ref)] @ bs @ [(zid, ref)] @ cs @ [(yid, Some xid)]) xid yid"
         using list_order_insert_ref assms(1) insert_ops_appendD split append.assoc None by metis
       hence "list_order ops xid yid"
@@ -1261,14 +1267,14 @@ proof(cases "xid < zid")
     next
       case (Some r)
       then show ?thesis
-      proof(cases "r \<in> set (interp_list as)")
+      proof(cases "r \<in> set (interp_ins as)")
         case True
         hence r_xid: "list_order (as @ [(xid, ref)]) r xid"
           using list_order_insert_ref assms(1) insert_ops_appendD split append.assoc Some by metis
-        hence "xid \<in> set (interp_list (as @ [(xid, ref)]))"
+        hence "xid \<in> set (interp_ins (as @ [(xid, ref)]))"
           using list_order_memb2 assms(1) split by metis
-        hence xid_in: "xid \<in> set (interp_list (as @ [(xid, ref)] @ bs @ [(zid, ref)] @ cs))"
-          using interp_list_monotonic assms(1) insert_ops_appendD split append.assoc by metis
+        hence xid_in: "xid \<in> set (interp_ins (as @ [(xid, ref)] @ bs @ [(zid, ref)] @ cs))"
+          using interp_ins_monotonic assms(1) insert_ops_appendD split append.assoc by metis
         moreover have "list_order (as @ [(xid, ref)] @ bs) r xid"
           using list_order_append r_xid assms(1) insert_ops_appendD split append.assoc by metis
         hence "list_order (as @ [(xid, ref)] @ bs @ [(zid, ref)]) zid xid"
@@ -1282,16 +1288,16 @@ proof(cases "xid < zid")
         ultimately show ?thesis by blast
       next
         case False
-        hence "xid \<notin> set (interp_list ops)"
-          using interp_list_ref_nonex assms(1) split Some by metis
-        moreover have "xid \<notin> set (interp_list (as @ [(xid, ref)] @ bs @ [(zid, ref)] @ cs))"
-          using interp_list_ref_nonex assms(1) insert_ops_appendD split append.assoc Some False by metis
-        hence "yid \<notin> set (interp_list ops)"
-          using interp_list_ref_nonex assms(1) split append.assoc by metis
-        moreover have "r \<notin> set (interp_list (as @ [(xid, ref)] @ bs))"
-          using interp_list_append_non_memb assms(1) insert_ops_appendD split append.assoc Some False by metis
-        hence "zid \<notin> set (interp_list ops)"
-          using interp_list_ref_nonex assms(1) split append.assoc Some by metis
+        hence "xid \<notin> set (interp_ins ops)"
+          using interp_ins_ref_nonex assms(1) split Some by metis
+        moreover have "xid \<notin> set (interp_ins (as @ [(xid, ref)] @ bs @ [(zid, ref)] @ cs))"
+          using interp_ins_ref_nonex assms(1) insert_ops_appendD split append.assoc Some False by metis
+        hence "yid \<notin> set (interp_ins ops)"
+          using interp_ins_ref_nonex assms(1) split append.assoc by metis
+        moreover have "r \<notin> set (interp_ins (as @ [(xid, ref)] @ bs))"
+          using interp_ins_append_non_memb assms(1) insert_ops_appendD split append.assoc Some False by metis
+        hence "zid \<notin> set (interp_ins ops)"
+          using interp_ins_ref_nonex assms(1) split append.assoc Some by metis
         ultimately show ?thesis by blast
       qed
     qed
@@ -1306,10 +1312,10 @@ next
   then show ?thesis
   proof(cases ref)
     case None
-    hence "zid \<in> set (interp_list (as @ [(zid, ref)]))"
-      using interp_list_last_None assms(1) split by metis
-    hence "zid \<in> set (interp_list (as @ [(zid, ref)] @ bs))"
-      using interp_list_monotonic assms(1) insert_ops_appendD split append.assoc by metis
+    hence "zid \<in> set (interp_ins (as @ [(zid, ref)]))"
+      using interp_ins_last_None assms(1) split by metis
+    hence "zid \<in> set (interp_ins (as @ [(zid, ref)] @ bs))"
+      using interp_ins_monotonic assms(1) insert_ops_appendD split append.assoc by metis
     hence xid_zid: "list_order (as @ [(zid, ref)] @ bs @ [(xid, ref)]) xid zid"
       using list_order_insert_none assms(1) insert_ops_appendD split append.assoc None by metis
     hence "list_order (as @ [(zid, ref)] @ bs @ [(xid, ref)] @ cs) xid zid"
@@ -1318,10 +1324,10 @@ next
       using list_order_insert_between assms(1) insert_ops_appendD split append.assoc by metis
     hence "list_order ops yid zid"
       using list_order_append assms(1) split append.assoc by metis
-    moreover have "xid \<in> set (interp_list (as @ [(zid, ref)] @ bs @ [(xid, ref)]))"
+    moreover have "xid \<in> set (interp_ins (as @ [(zid, ref)] @ bs @ [(xid, ref)]))"
       using list_order_memb1 xid_zid assms(1) split by metis
-    hence "xid \<in> set (interp_list (as @ [(zid, ref)] @ bs @ [(xid, ref)] @ cs))"
-      using interp_list_monotonic assms(1) insert_ops_appendD split append.assoc by metis
+    hence "xid \<in> set (interp_ins (as @ [(zid, ref)] @ bs @ [(xid, ref)] @ cs))"
+      using interp_ins_monotonic assms(1) insert_ops_appendD split append.assoc by metis
     hence "list_order (as @ [(zid, ref)] @ bs @ [(xid, ref)] @ cs @ [(yid, Some xid)]) xid yid"
       using list_order_insert_ref assms(1) insert_ops_appendD split append.assoc by metis
     hence "list_order ops xid yid"
@@ -1330,7 +1336,7 @@ next
   next
     case (Some r)
     then show ?thesis
-    proof(cases "r \<in> set (interp_list as)")
+    proof(cases "r \<in> set (interp_ins as)")
       case True
       hence "list_order (as @ [(zid, ref)]) r zid"
         using list_order_insert_ref assms(1) insert_ops_appendD split append.assoc Some by metis
@@ -1344,7 +1350,7 @@ next
         using list_order_insert_between assms(1) insert_ops_appendD split append.assoc by metis
       hence "list_order ops yid zid"
         using list_order_append assms(1) split append.assoc by metis
-      moreover have "xid \<in> set (interp_list (as @ [(zid, ref)] @ bs @ [(xid, ref)] @ cs))"
+      moreover have "xid \<in> set (interp_ins (as @ [(zid, ref)] @ bs @ [(xid, ref)] @ cs))"
         using list_order_memb1 xid_zid assms(1) split by metis
       hence "list_order (as @ [(zid, ref)] @ bs @ [(xid, ref)] @ cs @ [(yid, Some xid)]) xid yid"
         using list_order_insert_ref assms(1) insert_ops_appendD split append.assoc by metis
@@ -1353,16 +1359,16 @@ next
       ultimately show ?thesis by blast
     next
       case False
-      hence "zid \<notin> set (interp_list ops)"
-        using interp_list_ref_nonex assms(1) split Some by metis
-      moreover have r_notin: "r \<notin> set (interp_list (as @ [(zid, ref)] @ bs))"
-        using interp_list_append_non_memb assms(1) insert_ops_appendD split append.assoc Some False by metis
-      hence "xid \<notin> set (interp_list (as @ [(zid, ref)] @ bs @ [(xid, ref)] @ cs))"
-        using interp_list_ref_nonex assms(1) insert_ops_appendD split append.assoc Some by metis
-      hence "yid \<notin> set (interp_list ops)"
-        using interp_list_ref_nonex assms(1) split append.assoc by metis
-      moreover have "xid \<notin> set (interp_list ops)"
-        using interp_list_ref_nonex r_notin assms(1) split append.assoc Some by metis
+      hence "zid \<notin> set (interp_ins ops)"
+        using interp_ins_ref_nonex assms(1) split Some by metis
+      moreover have r_notin: "r \<notin> set (interp_ins (as @ [(zid, ref)] @ bs))"
+        using interp_ins_append_non_memb assms(1) insert_ops_appendD split append.assoc Some False by metis
+      hence "xid \<notin> set (interp_ins (as @ [(zid, ref)] @ bs @ [(xid, ref)] @ cs))"
+        using interp_ins_ref_nonex assms(1) insert_ops_appendD split append.assoc Some by metis
+      hence "yid \<notin> set (interp_ins ops)"
+        using interp_ins_ref_nonex assms(1) split append.assoc by metis
+      moreover have "xid \<notin> set (interp_ins ops)"
+        using interp_ins_ref_nonex r_notin assms(1) split append.assoc Some by metis
       ultimately show ?thesis by blast
     qed
   qed
