isabelle/RGA.thy
@@ -34,7 +34,7 @@ definition interp_rga :: "('oid::{linorder} \<times> 'oid option) list \<Rightar
   "interp_rga ops \<equiv> foldl insert_rga [] ops"
 
 
-subsection\<open>Commutativity of insert\_rga\<close>
+subsection\<open>Commutativity of \isa{insert-rga}\<close>
 
 lemma insert_body_set_ins [simp]:
   shows  "set (insert_body xs e) = insert e (set xs)"
@@ -179,10 +179,10 @@ next
 qed
 
 
-subsection\<open>Lemmata about the rga\_ops predicate\<close>
+subsection\<open>Lemmata about the \isa{rga-ops} predicate\<close>
 
 definition rga_ops :: "('oid::{linorder} \<times> 'oid option) list \<Rightarrow> bool" where
-  "rga_ops list \<equiv> crdt_ops set_option list"
+  "rga_ops list \<equiv> crdt_ops list set_option"
 
 lemma rga_ops_rem_last:
   assumes "rga_ops (xs @ [x])"
@@ -194,7 +194,7 @@ lemma rga_ops_rem_penultimate:
     and "\<And>r. r2 = Some r \<Longrightarrow> r \<noteq> i1"
   shows "rga_ops (xs @ [(i2, r2)])"
 using assms proof -
-  have "crdt_ops set_option (xs @ [(i2, r2)])"
+  have "crdt_ops (xs @ [(i2, r2)]) set_option"
     using assms crdt_ops_rem_penultimate rga_ops_def by fastforce
   thus "rga_ops (xs @ [(i2, r2)])"
     by (simp add: rga_ops_def)
@@ -204,7 +204,7 @@ lemma rga_ops_ref_exists:
   assumes "rga_ops (pre @ (oid, Some ref) # suf)"
   shows "ref \<in> fst ` set pre"
 proof -
-  from assms have "crdt_ops set_option (pre @ (oid, Some ref) # suf)"
+  from assms have "crdt_ops (pre @ (oid, Some ref) # suf) set_option"
     by (simp add: rga_ops_def)
   moreover have "set_option (Some ref) = {ref}"
     by simp
@@ -213,7 +213,7 @@ proof -
 qed
 
 
-subsection\<open>Lemmata about the interp\_rga function\<close>
+subsection\<open>Lemmata about the \isa{interp-rga} function\<close>
 
 lemma interp_rga_tail_unfold:
   shows "interp_rga (xs@[x]) = insert_rga (interp_rga (xs)) x"
@@ -286,8 +286,8 @@ lemma final_insert:
   assumes "set (xs @ [x]) = set (ys @ [x])"
     and "rga_ops (xs @ [x])"
     and "insert_ops (ys @ [x])"
-    and "interp_rga xs = interp_list ys"
-  shows "interp_rga (xs @ [x]) = interp_list (ys @ [x])"
+    and "interp_rga xs = interp_ins ys"
+  shows "interp_rga (xs @ [x]) = interp_ins (ys @ [x])"
 proof -
   obtain oid ref where x_pair: "x = (oid, ref)" by force
   have "distinct (xs @ [x])" and "distinct (ys @ [x])"
@@ -303,14 +303,14 @@ proof -
     thus "\<And>i. i \<in> set (interp_rga xs) \<Longrightarrow> i < oid"
       using assms(2) interp_rga_ids rga_ops_rem_last by blast
   qed
-  thus "interp_rga (xs @ [x]) = interp_list (ys @ [x])"
+  thus "interp_rga (xs @ [x]) = interp_ins (ys @ [x])"
   proof(cases ref)
     case None
     moreover from this have "insert_rga (interp_rga xs) (oid, ref) = oid # interp_rga xs"
       using oid_greatest hd_in_set insert_body.elims insert_body.simps(1)
         insert_rga.simps(1) list.sel(1) by metis
-    ultimately show "interp_rga (xs @ [x]) = interp_list (ys @ [x])" 
-      using assms(4) by (simp add: interp_list_tail_unfold interp_rga_tail_unfold x_pair)
+    ultimately show "interp_rga (xs @ [x]) = interp_ins (ys @ [x])" 
+      using assms(4) by (simp add: interp_ins_tail_unfold interp_rga_tail_unfold x_pair)
   next
     case (Some r)
     have "\<exists>as bs. interp_rga xs = as @ r # bs"
@@ -328,8 +328,8 @@ proof -
       by (metis as_bs insert_between_elements oid_greatest)
     moreover have "insert_spec (as @ r # bs) (oid, Some r) = as @ r # oid # bs"
       by (meson \<open>distinct (as @ r # bs)\<close> insert_after_ref)
-    ultimately show "interp_rga (xs @ [x]) = interp_list (ys @ [x])" 
-      by (metis assms(4) Some as_bs interp_list_tail_unfold interp_rga_tail_unfold x_pair)
+    ultimately show "interp_rga (xs @ [x]) = interp_ins (ys @ [x])" 
+      by (metis assms(4) Some as_bs interp_ins_tail_unfold interp_rga_tail_unfold x_pair)
   qed
 qed
 
@@ -379,23 +379,23 @@ lemma rga_spec_equal:
   assumes "set xs = set ys"
     and "insert_ops xs"
     and "rga_ops ys"
-  shows "interp_list xs = interp_rga ys"
+  shows "interp_ins xs = interp_rga ys"
 using assms proof(induction xs arbitrary: ys rule: rev_induct)
   case Nil
-  then show ?case by (simp add: interp_rga_def interp_list_def)
+  then show ?case by (simp add: interp_rga_def interp_ins_def)
 next
   case (snoc x xs)
   hence "x \<in> set ys"
     by (metis last_in_set snoc_eq_iff_butlast)
   from this obtain pre suf where ys_split: "ys = pre @ [x] @ suf"
     using split_list_first by fastforce
-  have IH: "interp_list xs = interp_rga (pre @ suf)"
+  have IH: "interp_ins xs = interp_rga (pre @ suf)"
   proof -
-    have "crdt_ops set_option (pre @ suf)"
+    have "crdt_ops (pre @ suf) set_option"
     proof -
-      have "crdt_ops set_option (pre @ [x] @ suf)"
+      have "crdt_ops (pre @ [x] @ suf) set_option"
         using rga_ops_def snoc.prems(3) ys_split by blast
-      thus "crdt_ops set_option (pre @ suf)"
+      thus "crdt_ops (pre @ suf) set_option"
         using crdt_ops_rem_spec snoc.prems ys_split insert_ops_def by blast
     qed
     hence "rga_ops (pre @ suf)"
@@ -408,13 +408,13 @@ next
   qed
   have valid_rga: "rga_ops (pre @ suf @ [x])"
   proof -
-    have "crdt_ops set_option (pre @ suf @ [x])"
+    have "crdt_ops (pre @ suf @ [x]) set_option"
       using snoc.prems ys_split
       by (simp add: crdt_ops_reorder_spec insert_ops_def rga_ops_def)
     thus "rga_ops (pre @ suf @ [x])"
       by (simp add: rga_ops_def)
   qed
-  have "interp_list (xs @ [x]) = interp_rga (pre @ suf @ [x])"
+  have "interp_ins (xs @ [x]) = interp_rga (pre @ suf @ [x])"
   proof -
     have "set (xs @ [x]) = set (pre @ suf @ [x])"
       using snoc.prems(1) ys_split by auto
@@ -436,7 +436,7 @@ next
     ultimately show "interp_rga (pre @ suf @ [x]) = interp_rga (pre @ [x] @ suf)"
       using interp_rga_reorder valid_rga x_pair by force
   qed
-  ultimately show "interp_list (xs @ [x]) = interp_rga ys"
+  ultimately show "interp_ins (xs @ [x]) = interp_rga ys"
     by (simp add: ys_split)
 qed
 
@@ -474,7 +474,7 @@ next
   proof -
     have "\<forall>r \<in> set_option ref. r < oid"
       using calculation(3) crdt_ops_ref_less_last rga_ops_def snoc.prems by fastforce
-    hence "spec_ops set_option (pre @ [(oid, ref)] @ suf)"
+    hence "spec_ops (pre @ [(oid, ref)] @ suf) set_option"
       using spec_ops_add_any calculation insert_ops_def by metis
     thus ?thesis by (simp add: insert_ops_def)
   qed
@@ -484,7 +484,7 @@ qed
 
 theorem rga_meets_spec:
   assumes "rga_ops xs"
-  shows "\<exists>ys. set ys = set xs \<and> insert_ops ys \<and> interp_list ys = interp_rga xs"
+  shows "\<exists>ys. set ys = set xs \<and> insert_ops ys \<and> interp_ins ys = interp_rga xs"
   using assms rga_spec_equal insert_ops_exist by metis
 
 end
